\makeheading{Lecture 19}{\printdate{2023-03-20}}%chktex 8
\section{Lecture 19}
\begin{itemize}
    \item $ n_{..}=\sum_{i}\sum_j n_{ij} $
    \item $ \Vector{n}_{a.}=(n_{1.},\ldots,n_{a.})' $.
    \item $ \Vector{n}_{.b}=(n_{.1},\ldots,n_{.b})' $.
    \item $ \Matrix{D}_{a.}=\diag{n_{1.},\ldots,n_{a.}} $.
    \item $ \Matrix{D}_{.b}=\diag{n_{.1},\ldots,n_{.b}} $.
    \item $ \Matrix{N}=\begin{pmatrix}
                  n_{11} & \cdots & n_{1(b-1)} \\
                  \vdots & \ddots & \vdots     \\
                  n_{a1} & \cdots & n_{a(b-1)}
              \end{pmatrix} $.
    \item $ \Vector{n}_{.b}=\begin{pmatrix}
                  n_{1b} \\
                  \vdots \\
                  n_{ab}
              \end{pmatrix} $.
\end{itemize}
\[ \Matrix{X}'\Matrix{X}=\begin{pmatrix}
        n_{..}              & \Vector{n}_{a.}' & \Vector{n}_{.(b-1)}' & n_{.b}       \\
        \Vector{n}_{a.}     & \Matrix{D}_{a.}  & \Matrix{N}           & \Vector{n}_b \\
        \Vector{n}_{.(b-1)} & \Matrix{N}       & \Matrix{D}_{.(b-1)}  & \Matrix{O}   \\
        n_{.b}              & \Vector{n}_{b}'  & \Matrix{O}           & n_{.b}
    \end{pmatrix}. \]
A $ g $-inverse of $ \Matrix{X}'\Matrix{X} $ is
\[ \Matrix{F}=\begin{pmatrix}
        \Matrix{O} & \Matrix{O}                                                & \Matrix{O}                 & \Matrix{O} \\
        \Matrix{O} & \Matrix{D}_{a.}^{-1}+\Matrix{M}\Matrix{C}^{-1}\Matrix{M}' & -\Matrix{M}\Matrix{C}^{-1} & \Matrix{O} \\
        \Matrix{O} & -\Matrix{C}^{-1}\Matrix{M}'                               & \Matrix{C}^{-1}            & \Matrix{O} \\
        \Matrix{O} & \Matrix{O}                                                & \Matrix{O}                 & \Matrix{O} \\
    \end{pmatrix}. \]
\begin{align*}
    \Matrix{F}\Matrix{X}'\Matrix{X}
     & =\begin{pmatrix}
            \Matrix{O} & \Matrix{O} & \Matrix{O} & \Matrix{O} \\
            \boxed{1}  & \boxed{5}  & \boxed{6}  & \boxed{3}  \\
            \boxed{2}  & \boxed{7}  & \boxed{8}  & \boxed{4}  \\
            \Matrix{O} & \Matrix{O} & \Matrix{O} & \Matrix{O}
        \end{pmatrix}.
\end{align*}
\begin{align*}
    \boxed{1}
     & =(\Matrix{D}_{a.}^{-1}+\Matrix{M}\Matrix{C}^{-1}\Matrix{M}')\Vector{n}_{a.}-\Matrix{M}\Matrix{C}'\Vector{n}_{.(b-1)} \\
     & =\Matrix{D}_{a.}^{-1}\Vector{n}_{a.}+\Matrix{M}\Matrix{C}^{-1}[\Matrix{M}'\Vector{n}_{a.}-\Vector{n}_{.(b-1)}]       \\
     & =\Vector{j}_a+\Matrix{M}\Matrix{C}^{-1}\Matrix{O}                                                                    \\
     & =\Vector{j}_a.
\end{align*}
\begin{align*}
    \Matrix{M}
    =\Matrix{D}_{a.}^{-1}\Matrix{N}
    \implies \Matrix{M}'\Vector{n}_{a.} & =\Matrix{N}'\Matrix{D}_{a.}^{-1}\Vector{n}_{a.} \\
                                        & =\Matrix{N}'\Vector{j}_a                        \\
                                        & =\begin{pmatrix}
                                               n_{11} & \cdots & n_{1(b-1)} \\
                                               \vdots & \ddots & \vdots     \\
                                               n_{a1} & \cdots & n_{a(b-1)}
                                           \end{pmatrix}\begin{pmatrix}
                                                            1      \\
                                                            \vdots \\
                                                            1
                                                        \end{pmatrix}                   \\
                                        & =\begin{pmatrix}
                                               n_{.1} \\
                                               \vdots \\
                                               n_{.(b-1)}
                                           \end{pmatrix}.
\end{align*}

\begin{align*}
    \boxed{2}
     & =-\Matrix{C}^{-1}\Matrix{M}'\Vector{n}_{a.}+\Matrix{C}^{-1}\Vector{n}_{.(b-1)} \\
     & =-\Matrix{C}^{-1}[\Matrix{M}'\Vector{n}_{a.}-\Vector{n}_{.(b-1)}]              \\
     & =\Matrix{O}.
\end{align*}
\begin{align*}
    \boxed{5}
     & =(\Matrix{D}_{a.}^{-1}+\Matrix{M}\Matrix{C}^{-1}\Matrix{M}')\Matrix{D}_{a.}-\Matrix{M}\Matrix{C}^{-1}\Matrix{N}'              \\
     & =\Matrix{D}_{a.}^{-1}\Matrix{D}_{a.}+\Matrix{M}\Matrix{C}^{-1}\Matrix{M}'\Matrix{D}_{a.}-\Matrix{M}\Matrix{C}^{-1}\Matrix{N}' \\
     & =\Matrix{I}_a+\Matrix{M}\Matrix{C}^{-1}[\Matrix{M}'\Matrix{D}_{a.}-\Matrix{N}']                                               \\
     & =\Matrix{I}_a.
\end{align*}
\begin{align*}
    \Matrix{M}'
     & =\Matrix{N}'\Matrix{D}_{a.}^{-1}.               \\
    \implies \Matrix{M}'\Matrix{D}_a
     & =\Matrix{N}'\Matrix{D}_{a.}^{-1}\Matrix{D}_{a.} \\
     & =\Matrix{N}'
\end{align*}
\begin{align*}
    \boxed{6}
     & =(\Matrix{D}_{a.}^{-1}+\Matrix{M}\Matrix{C}^{-1}\Matrix{M}')\Matrix{N}-\Matrix{M}\Matrix{C}^{-1}\Matrix{D}_{.(b-1)}         \\
     & =\Matrix{D}_{a.}^{-1}\Matrix{N}+\Matrix{M}\Matrix{C}^{-1}\Matrix{M}'\Matrix{N}-\Matrix{M}\Matrix{C}^{-1}\Matrix{D}_{.(b-1)} \\
     & =\Matrix{M}+\Matrix{M}\Matrix{C}^{-1}(\Matrix{M}'\Matrix{N}-\Matrix{D}_{.(b-1)})                                            \\
     & =\Matrix{M}-\Matrix{M}\Matrix{C}^{-1}\Matrix{C}                                                                             \\
     & =\Matrix{O}.
\end{align*}
\[ \Matrix{C}=\Matrix{D}_{.(b-1)}-\Matrix{N}'\Matrix{D}_{a.}^{-1}\Matrix{N}=\Matrix{D}_{.(b-1)}-\Matrix{M}'\Matrix{N}. \]
\begin{align*}
    \boxed{7}
     & =-\Matrix{C}^{-1}\Matrix{M}'\Matrix{D}_{a.}+\Matrix{C}^{-1}\Matrix{N}' \\
     & =-\Matrix{C}^{-1}[\Matrix{M}'\Matrix{D}_{a.}-\Matrix{N}']              \\
     & =-\Matrix{C}^{-1}\Matrix{O}                                            \\
     & =\Matrix{O}.
\end{align*}
\begin{align*}
    \boxed{8}
     & =-\Matrix{C}^{-1}\Matrix{M}'\Matrix{N}+\Matrix{C}^{-1}\Matrix{D}_{.(b-1)} \\
     & =-\Matrix{C}^{-1}(\Matrix{D}_{.(b-1)}-\Matrix{M}'\Matrix{N})              \\
     & =\Matrix{C}^{-1}\Matrix{C}                                                \\
     & =\Matrix{I}_{b-1}.
\end{align*}
\begin{align*}
    \boxed{3}
     & =(\Matrix{D}_{.(b-1)}^{-1}+\Matrix{M}\Matrix{C}^{-1}\Matrix{M}')\Vector{n}_{b}                           \\
     & =(\Matrix{D}_{a.}^{-1}+\Matrix{M}\Matrix{C}^{-1}\Matrix{M}')(\Vector{n}_{a.}-\Matrix{N}\Vector{j}_{b-1}) \\
     & =\Matrix{D}_{a.}^{-1}\Vector{n}_{a.}+\Matrix{M}\Matrix{C}^{-1}\Matrix{M}'\Vector{n}_{a.}                 \\
     & \quad-(\Matrix{D}_{a.}^{-1}+\Matrix{M}\Matrix{C}^{-1}\Matrix{M}')\Matrix{N}\Vector{j}_{b-1}              \\
     & =\Vector{j}_a+\Matrix{M}\Matrix{C}^{-1}\Matrix{N}'\Matrix{D}_{a.}^{-1}\Vector{n}_{a.}                    \\
     & \quad-(\Matrix{D}_{a.}^{-1}+\Matrix{M}\Matrix{C}^{-1}\Matrix{M}')\Matrix{N}\Vector{j}_{b-1}              \\
     & =\Vector{j}_{a.}+\Matrix{M}\Matrix{C}^{-1}\Vector{j}_a+                                                  \\
     & \quad-\Matrix{M}\Matrix{C}^{-1}\Matrix{D}_{.(b-1)}\Vector{j}_{b-1}                                       \\
     & =\Vector{j}_a+\Matrix{M}\Matrix{C}^{-1}[\Matrix{N}'\Vector{j}_a-\Matrix{D}_{.(b-1)}\Vector{j}_{b-1}]     \\
     & =\Vector{j}_a+\Matrix{M}\Matrix{C}^{-1}\left(\begin{pmatrix}
                                                            n_{.1} \\
                                                            \vdots \\
                                                            n_{.(b-1)}
                                                        \end{pmatrix}-\begin{pmatrix}
                                                                          n_{.1} \\
                                                                          \vdots \\
                                                                          n_{.(b-1)}
                                                                      \end{pmatrix}\right)                          \\
     & =\Vector{j}_a.
\end{align*}
\begin{align*}
    \Vector{n}_{.a}
     & =\begin{pmatrix}
            n_{1.} \\
            \vdots \\
            n_{a.}
        \end{pmatrix}
    =\begin{pmatrix}
         n_{11}+\cdots+n_{1(b-1)}+n_{1b} \\
         \vdots                          \\
         n_{a1}+\cdots+n_{a(b-1)}+n_{ab}
     \end{pmatrix}               \\
     & =\Matrix{N}\Vector{j}_{b-1}+\Vector{n}_{b}.
\end{align*}
\begin{align*}
    (\Matrix{D}_{a.}^{-1}+\Matrix{M}\Matrix{C}^{-1}\Matrix{M}')\Matrix{N}-\Matrix{M}\Matrix{C}^{-1}\Matrix{D}_{.(b-1)}
     & =\Matrix{D}_{a.}^{-1}\Matrix{N}+\Matrix{M}\Matrix{C}^{-1}\Matrix{M}'\Matrix{N}-\Matrix{M}\Matrix{C}^{-1}\Matrix{D}_{.(b-1)} \\
     & =\Matrix{M}-\Matrix{M}\Matrix{C}^{-1}(\Matrix{D}_{.(b-1)}-\Matrix{M}'\Matrix{N})                                            \\
     & =\Matrix{M}-\Matrix{M}                                                                                                      \\
     & =\Matrix{O}
\end{align*}
\begin{align*}
    \boxed{4}
     & =-\Matrix{C}^{-1}\Matrix{M}'\Vector{n}_{b}                                                                        \\
     & =-\Matrix{C}^{-1}\Matrix{M}'[\Vector{n}_{a.}-\Matrix{N}\Vector{j}_{b-1}]                                          \\
     & =-\Matrix{C}^{-1}\Matrix{M}'\Vector{n}_{a.}+\Matrix{C}^{-1}\Matrix{M}'\Matrix{N}\Vector{j}_{b-1}                  \\
     & =-\Matrix{C}^{-1}\Matrix{M}'\Vector{n}_{a.}+(\Matrix{C}^{-1}\Matrix{D}_{.(b-1)}-\Matrix{I}_{b-1})\Vector{j}_{b-1} \\
     & =-\Matrix{C}^{-1}\Matrix{M}'\Vector{n}_{a.}+\Matrix{C}^{-1}\Matrix{D}_{.(b-1)}\Vector{j}_{b-1}-\Vector{j}_{b-1}   \\
     & =-\Matrix{C}^{-1}[\Matrix{M}'\Vector{n}_{a.}-\Matrix{D}_{.(b-1)}\Vector{j}_{b-1}]-\Vector{j}_{b-1}                \\
     & =-\Matrix{C}^{-1}\Matrix{O}-\Vector{j}_{b-1}                                                                      \\
     & =-\Vector{j}_{b-1}.
\end{align*}
Therefore,
\[ \Matrix{F}\Matrix{X}'\Matrix{X}
    =\begin{pmatrix}
        \Matrix{O}   & \Matrix{O}   & \Matrix{O}       & \Matrix{O}        \\
        \Vector{j}_a & \Matrix{I}_a & \Matrix{O}       & \Vector{j}_a      \\
        \Matrix{O}   & \Matrix{O}   & \Matrix{I}_{b-1} & -\Vector{j}_{b-1} \\
        \Matrix{O}   & \Matrix{O}   & \Matrix{O}       & \Matrix{O}
    \end{pmatrix}. \]
\subsection*{Estimable Combinations}
$ \Matrix{W}'\Matrix{F}\Matrix{X}'\Matrix{X}=\Matrix{W} $,
where
\[ \Matrix{W}=\begin{pmatrix}
        w_0 & w_1 & \cdots & w_a & w_{a+1} & \cdots & w_{a+b}
    \end{pmatrix}. \]
\begin{align*}
    W'\Vector{\beta}
     & =w_0\mu+w_1\alpha_1+\cdots+w_a\alpha_a+w_{a+1}\beta_1+\cdots+w_{a+b}\beta_b        \\
     & =(w_1+\cdots+w_a)\mu+w_1\alpha_1+\cdots+w_a\alpha_a                                \\
     & \quad+ w_{a+1}\beta_1+\cdots+w_{a+b-1}\beta_{b-1}                                  \\
     & \quad+\bigl[(w_1+\cdots+w_a)-(w_{a+1}+\cdots+w_{a+b-1})\bigr]\beta_b               \\
     & =\sum_{i=1}^{a}w_i(\mu+\alpha_i+\beta_b)+\sum_{j=1}^{b-1}w_{j+a}(\beta_j-\beta_b).
\end{align*}
\begin{align*}
    \Matrix{W}'\begin{pmatrix}
                   \Matrix{O}   & \Matrix{O}   & \Matrix{O}       & \Matrix{O}        \\
                   \Vector{j}_a & \Matrix{I}_a & \Matrix{O}       & \Vector{j}_a      \\
                   \Matrix{O}   & \Matrix{O}   & \Matrix{I}_{b-1} & -\Vector{j}_{b-1} \\
                   \Matrix{O}   & \Matrix{O}   & \Matrix{O}       & \Matrix{O}
               \end{pmatrix}
     & =\begin{pmatrix}
            w_1+\cdots+w_a                          \\
            w_1+\cdots+w_a+w_{a+1}+\cdots+a_{a+b-1} \\
            (w_1+\cdots+w_a)-(w_{a+1}+\cdots+w_{a+b+-1})
        \end{pmatrix}'
\end{align*}
Therefore,
\begin{align*}
    w_0     & =w_1+\cdots+w_a.                            \\
    w_{a+b} & =w_1+\cdots+w_a-(w_{a+1}+\cdots+w_{a+b-1}).
\end{align*}
\begin{enumerate}[(1)]
    \item $ \mu+\alpha_k+\beta_\ell $ is estimable. $ w_k=w_{\ell+a}=1 $ for $ \ell<b $, and $ w_k=1 $ otherwise.
    \item $ \alpha_k-\alpha_\ell $ is estimable.
    \item $ \beta_k-\beta_\ell $ is estimable.
    \item $ \beta_k+\frac{1}{n_{.k}}\sum_{i=1}^{a}n_{ik}\alpha_i\sim _{.k}\beta_k+\sum_{i=1}^{a}n_{ik}\alpha_i $ is estimable.
    \item $ \alpha_\ell+\frac{1}{n_{\ell.}}\sum_{j=1}^{b}n_{\ell j}\beta_j $ is estimable.
\end{enumerate}